experiment/Experiment.Steel.Tac.LV.fst
@@ -202,6 +202,9 @@ let __build_LCret
 /// By independence of [g_csm], we mean that the consumption of a [vprop'] cannot depend on [x], the [vprop']
 /// themselves are necessarily independent of [x] since they are from [env].
 /// We use a [LCsub] on [g] to force the consumption of [f_prd]. The independence is ensured by [eqs].
+/// We declare [g_csm] with type [list bool] instead of [csm_t (filter_mask (mask_not f_csm) env)] so that
+/// we can check by tactic (using [g_csm_len] that it has the correct length). Otherwise this proof obligation
+/// could be sent to the SMT.
 [@@ __cond_solver__]
 let __build_LCbind
       (env : vprop_list)
@@ -210,15 +213,17 @@ let __build_LCbind
       (cf : lin_cond env f f_csm f_prd)
       (g_csm0 : (x : a) -> csm_t (res_env env f_csm (f_prd x))) (g_prd0 : (x : a) -> prd_t b)
       (cg : (x : a) -> lin_cond (res_env env f_csm (f_prd x)) (g x) (g_csm0 x) (g_prd0 x))
-      (g_csm : csm_t (filter_mask (mask_not f_csm) env)) (g_prd : prd_t b)
+      (g_csm : list bool) (g_prd : prd_t b)
       (eqs : (x : a) -> squash (
             let n0 = L.length (f_prd x) in
             (**) L.splitAt_length n0 (g_csm0 x);
             let g_csm0_f_prd : Ll.vec n0 bool = (L.splitAt n0 (g_csm0 x))._1 in
             eq2 #(list bool) g_csm (L.splitAt (L.length (f_prd x)) (g_csm0 x))._2 /\
             g_prd == (fun (y : b) -> L.(g_prd0 x y @ filter_mask (mask_not g_csm0_f_prd) (f_prd x)))))
+      (g_csm_len : squash (L.length g_csm == mask_len (mask_not f_csm)))
   : lin_cond u#a u#p env (M.Tbind a b f g) (bind_csm env f_csm g_csm) g_prd
   =
+    let g_csm : csm_t (filter_mask (mask_not f_csm) env) = g_csm in
     LCbind env #a #b #f #g
       f_csm f_prd cf
       g_csm g_prd
@@ -280,10 +285,11 @@ let __build_LCbindP
       (a : Type) (b : Type) (wp : pure_wp a) (g : a -> M.prog_tree b)
       (csm0 : (x : a) -> csm_t env) (prd0 : (x : a) -> prd_t b)
       (cg : (x : a) -> lin_cond env (g x) (csm0 x) (prd0 x))
-      (csm : csm_t env) (prd : prd_t b)
+      (csm : list bool) (prd : prd_t b)
       // Since we use [__defer_sig_unification], it is probably not necessary to do this indirection,
       // but it allows to point the dependency on x in the failure message
-      (eqs : (x : a) -> squash (csm == csm0 x /\ prd == prd0 x))
+      (eqs : (x : a) -> squash (eq2 #(list bool) csm (csm0 x) /\ prd == prd0 x))
+      (csm_len : squash (L.length csm == L.length env))
   : lin_cond u#a u#p env (M.TbindP a b wp g) csm prd
   =
     LCbindP env #a #b #wp #g csm prd (fun x -> eqs x; cg x)
@@ -389,8 +395,12 @@ let rec build_LCbind fr ctx prd_hint_b : Tac unit
     norm_lc ();
     split ();
       let ctx = ctx_set_loc ctx "in the bind statement" in
-      cs_try trefl fr ctx (fun m -> fail (m (Fail_dependency "csm" x) []));
-      cs_try trefl fr ctx (fun m -> fail (m (Fail_dependency "prd" x) []))
+      cs_try (fun () -> unify_recheck SMT) fr ctx (fun m -> fail (m (Fail_dependency "csm" x) []));
+      // If there is some subtyping in the vprop it will be re-sent to the SMT. ALT? use Force instead
+      cs_try (fun () -> unify_recheck SMT) fr ctx (fun m -> fail (m (Fail_dependency "prd" x) []));
+    // [g_csm_len]
+    norm_lc ();
+    trefl ()
 
 and build_LCbindP fr ctx prd_hint_b : Tac unit
   =
@@ -398,14 +408,16 @@ and build_LCbindP fr ctx prd_hint_b : Tac unit
     // cg
     let x = intro () in
     build_lin_cond fr (ctx_path_node ctx 0) prd_hint_b;
-    // 
-    // [g_csm <- ...], [g_prd <- ...]
+    // [csm <- ...], [prd <- ...]
     let x = intro () in
     norm_lc ();
     split ();
       let ctx = ctx_set_loc ctx "in the bindP statement" in
-      cs_try trefl fr ctx (fun m -> fail (m (Fail_dependency "csm" x) []));
-      cs_try trefl fr ctx (fun m -> fail (m (Fail_dependency "prd" x) []))
+      cs_try (fun () -> unify_recheck SMT) fr ctx (fun m -> fail (m (Fail_dependency "csm" x) []));
+      cs_try (fun () -> unify_recheck SMT) fr ctx (fun m -> fail (m (Fail_dependency "prd" x) []));
+    // csm_len
+    norm_lc ();
+    trefl ()
 
 and build_LCif fr ctx prd_hint_b : Tac unit
   =
@@ -445,7 +457,7 @@ and build_lin_cond (fr : flags_record) (ctx : cs_context) (prd_hint_b : option b
     build_tac fr ctx prd_hint_b;
     // [?csm0 <- csm1], [?prd0 <- prd1]
     norm_lc ();
-    split (); trefl (); trefl ()
+    split (); trefl (); trefl () // unify_recheck should not be needed since we do not change the context
 
 #push-options "--ifuel 0 --fuel 0"
 [@@ __cond_solver__]
